\documentclass{ximera}

\author{Anna Davis} \title{MTH 160 Homework 3} 

\begin{document}

\begin{abstract}

\end{abstract}
\maketitle
 \textit{Certificate due: 2/3/2021 at 11:59 p.m.}
 
 \section{Lecture 4}
\begin{problem}\label{prob:160hom2prob6}
Let $f(x)=2x^2-x$ and $g(x)=-x^2+3$.  Evaluate each expression.
\begin{enumerate}
    \item $(f\circ g)(0)=\answer{15}$
    \item $(f\circ g)(2)=\answer{3}$
    \item $(f\circ g)(-3)=\answer{78}$
    \item $(g\circ f)(0)=\answer{3}$
    \item $(g\circ f)(-1)=\answer{-6}$
    \item $(f\circ f)(2)=\answer{66}$
    \item $(g\circ g)(-2)=\answer{2}$
\end{enumerate}
\end{problem}

\begin{problem}\label{prob:160hom2prob7}
The graphs of $f$ and $g$ are shown.  Use the graphs to evaluate each expression.
\begin{image}
   \includegraphics[height=1in]{160H2pic8.jpg}
 \end{image}
  \begin{enumerate}
\item
$(g\circ f)(2)=\answer{5}$

\item
$(f\circ g)(0)=\answer{4}$

  \end{enumerate}
\end{problem}
\begin{problem}\label{prob:160hom2prob8}
Let $f(x)=-3x^2-2x+1$ and $g(x)=4x-1$.  Evaluate each expression and simplify as much as possible.
\begin{enumerate}
    \item $(g\circ f)(x)=\answer{-12}x^2-\answer{8}x+\answer{3}$
    \item $(f\circ g)(x)=\answer{-48}x^2+\answer{16}x$
    \item $(g\circ g)(x)=\answer{16x-5}$ (Enter symbolic expression containing $x$.)
\end{enumerate}
\end{problem}
 
 \section{Lectures 5 and 6}
\begin{problem}\label{prob:160hom3prob1}
For each given function $g$, identify the "base function" $f$, and select the transformations applied to the graph of $f$ to obtain the graph of $g$.
\begin{enumerate}
    \item $g(x)=-x^2+1$
    
    Base function:  $f(x)=\answer{x^2}$
    \begin{multipleChoice}  
\choice{Reflection about the $x$-axis; Horizontal shift to the right by 1 unit.}
\choice[correct]{Reflection about the $x$-axis; Vertical shift up by 1 unit.}  
\choice{Reflection about the $y$-axis; Vertical shift down by 1 unit.}  
\choice{Horizontal shift to the left by 1 unit.}  
\end{multipleChoice}
\item $g(x)=\frac{1}{x}+2$
    
    Base function:  $f(x)=\answer{\frac{1}{x}}$
    \begin{multipleChoice}  
\choice{Horizontal shift to the right by 2 units.}
\choice{Horizontal shift to the left by 2 units.}
\choice[correct]{Vertical shift upwards by 2 units.}  
\choice{Vertical shift downwards by 2 units.}  
  \end{multipleChoice}
  \item $g(x)=\sqrt{x+3}-1$
    
    Base function:  $f(x)=\answer{\sqrt{x}}$
    \begin{multipleChoice}  
    \choice{Vertical shift upwards by 3 units; Vertical shift downwards by 1 unit.}  
\choice{Horizontal shift to the right by 3 units; Vertical shift downwards by 1 unit.}
\choice{Horizontal shift to the left by 3 units; Vertical shift upwards by 1 unit.}
\choice[correct]{Horizontal shift to the left by 3 units; Vertical shift downwards by 1 unit.}  
  \end{multipleChoice}
  \item $g(x)=-\frac{1}{x-4}$
    
    Base function:  $f(x)=\answer{\frac{1}{x}}$
    \begin{multipleChoice}  
 \choice[correct]{Horizontal shift to the right by 4 units; Reflection about the $x$-axis.}
\choice{Horizontal shift to the left by 4 units; Reflection about the $x$-axis.}
\choice{Vertical shift upwards by 4 units; Reflection about the $x$-axis.} 
\choice{Reflection about the $y$-axis.  Vertical shift downwards by 4 units.}  
  \end{multipleChoice}
\end{enumerate}
\end{problem}
\begin{problem}\label{prob:160hom3prob2}
The graphs of function $f$ (in red) and function $g$ (in blue) are given. Express $g$ in terms of $f$.
\begin{enumerate}
    \item \begin{image}
   \includegraphics[height=1in]{160H3pic4.jpg}
 \end{image}
 \begin{multipleChoice}  
 \choice[correct]{$g(x)=2f(x)$}
\choice{$g(x)=f(x)+2$}
\choice{$g(x)=f(x-2)$} 
\choice{$g(x)=f(x+2)$}  
  \end{multipleChoice}
  
   \item \begin{image}
   \includegraphics[height=1in]{160H3pic2.jpg}
 \end{image}
 \begin{multipleChoice}  
 \choice{$g(x)=-f(x)-1$}
\choice{$g(x)=-f(x-1)$} 
\choice{$g(x)=-f(x+1)$}  
\choice[correct]{$g(x)=-f(x)+1$}
  \end{multipleChoice}
  
  \item \begin{image}
   \includegraphics[height=1in]{160H3pic3.jpg}
 \end{image}
 \begin{multipleChoice}  
 \choice{$g(x)=-f(x+1)-1$}
 \choice[correct]{$g(x)=-f(x-1)+1$}
\choice{$g(x)=-f(x-1)-1$} 
\choice{$g(x)=f(x+1)$}  
  \end{multipleChoice}
\end{enumerate}
\end{problem}

\end{document} 